code/experimental/P256/Hacl.Spec.P256.MontgomeryMultiplication.fst
@@ -729,4 +729,52 @@ let exponent a result tempBuffer =
   big_power k ((pow2 32 - 1) * pow2 224) (pow2 192) ((pow2 94 -1 ) * pow2 2) 1;
   assert_norm(((pow2 32 - 1) * pow2 224 + pow2 192 + (pow2 94 -1 ) * pow2 2 + 1) = prime - 2)
 
+(*This code is taken from Curve25519, written by Polubelova M *)
+val lemma_cswap2_step:
+    bit:uint64{v bit <= 1}
+  -> p1:uint64
+  -> p2:uint64
+  -> Lemma (
+      let mask = u64 0 -. bit in
+      let dummy = mask &. (p1 ^. p2) in
+      let p1' = p1 ^. dummy in
+      let p2' = p2 ^. dummy in
+      if v bit = 1 then p1' == p2 /\ p2' == p1 else p1' == p1 /\ p2' == p2)
+let lemma_cswap2_step bit p1 p2 =
+  let mask = u64 0 -. bit in
+  assert (v bit == 0 ==> v mask == 0);
+  assert (v bit == 1 ==> v mask == pow2 64 - 1);
+  let dummy = mask &. (p1 ^. p2) in
+  logand_lemma mask (p1 ^. p2);
+  assert (v bit == 1 ==> v dummy == v (p1 ^. p2));
+  assert (v bit == 0 ==> v dummy == 0);
+  let p1' = p1 ^. dummy in
+  uintv_extensionality dummy (if v bit = 1 then (p1 ^. p2) else u64 0);
+  logxor_lemma p1 p2;
+  let p2' = p2 ^. dummy in
+  logxor_lemma p2 p1
     
+let cswap bit p1 p2 =
+  let h0 = ST.get () in
+  let mask = u64 0 -. bit in
+
+  [@ inline_let]
+  let inv h1 (i:nat{i <= 8}) =
+    (forall (k:nat{k < i}).
+      if v bit = 1
+      then (as_seq h1 p1).[k] == (as_seq h0 p2).[k] /\ (as_seq h1 p2).[k] == (as_seq h0 p1).[k]
+      else (as_seq h1 p1).[k] == (as_seq h0 p1).[k] /\ (as_seq h1 p2).[k] == (as_seq h0 p2).[k]) /\
+    (forall (k:nat{i <= k /\ k < 8}).
+      (as_seq h1 p1).[k] == (as_seq h0 p1).[k] /\ (as_seq h1 p2).[k] == (as_seq h0 p2).[k]) /\
+    modifies (loc p1 |+| loc p2) h0 h1 in
+
+  Lib.Loops.for 0ul 12ul inv
+    (fun i ->
+      let dummy = mask &. (p1.(i) ^. p2.(i)) in
+      p1.(i) <- p1.(i) ^. dummy;
+      p2.(i) <- p2.(i) ^. dummy;
+      lemma_cswap2_step bit ((as_seq h0 p1).[v i]) ((as_seq h0 p2).[v i])
+    );
+  let h1 = ST.get () in
+  Lib.Sequence.eq_intro (as_seq h1 p1) (if v bit = 1 then as_seq h0 p2 else as_seq h0 p1);
+  Lib.Sequence.eq_intro (as_seq h1 p2) (if v bit = 1 then as_seq h0 p1 else as_seq h0 p2)
