code/experimental/P256/Hacl.Spec.P256.MontgomeryMultiplication.fsti
@@ -109,3 +109,15 @@ val exponent: a: felem ->result: felem -> tempBuffer: lbuffer uint64 (size 20) -
   disjoint a tempBuffer /\ as_nat h a < prime)
   (ensures fun h0 _ h1 -> modifies2 result tempBuffer h0 h1 /\ (let k = fromDomain_ (as_nat h0 a) in 
     as_nat h1 result =  toDomain_ ((pow k (prime-2)) % prime)))
+
+
+[@ CInline]
+val cswap: bit:uint64{v bit <= 1} -> p1:point -> p2:point
+  -> Stack unit
+    (requires fun h ->
+      live h p1 /\ live h p2 /\
+      (disjoint p1 p2 \/ p1 == p2))
+    (ensures  fun h0 _ h1 ->
+      modifies (loc p1 |+| loc p2) h0 h1 /\
+      (v bit == 1 ==> as_seq h1 p1 == as_seq h0 p2 /\ as_seq h1 p2 == as_seq h0 p1) /\
+      (v bit == 0 ==> as_seq h1 p1 == as_seq h0 p1 /\ as_seq h1 p2 == as_seq h0 p2))
